Griotte Assembler (#52)
* Re-introduce the assembler (added in (#11), but removed (#35))

* Re-implements the switcher (and the macros it uses) with Griotte assembler

* Make switcher a but more readable

* Clearing registers

* Nit: simplify dom_arg_rmap

* Fetch and assert macros with assembler

theories/switcher/clear_registers.v
@@ -1,171 +1,51 @@
-From iris.algebra Require Import frac.
-From iris.proofmode Require Import proofmode.
-From cap_machine Require Import memory_region rules proofmode.
-From iris.program_logic Require Export weakestpre.
-From cap_machine Require Export cap_lang seal_store region_invariants.
-From iris.algebra Require Export gmap agree auth excl_auth.
-From iris.base_logic Require Export invariants na_invariants saved_prop.
-From cap_machine Require Import rules_base.
+From cap_machine Require Import machine_parameters assembler.
 
-Section ClearRegistersMacro.
-  Context
-    {Σ:gFunctors}
-    {ceriseg:ceriseG Σ}
-    {sealsg: sealStoreG Σ}
-    {Cname : CmptNameG}
-    {stsg : STSG Addr region_type Σ}
-    {heapg : heapGS Σ}
-    `{MP: MachineParameters}.
+Section ClearStackMacro.
+  Import Asm_Griotte.
+  Local Coercion Z.of_nat : nat >-> Z.
+  Context `{MP: MachineParameters}.
 
-  Implicit Types W : WORLD.
-  Implicit Types C : CmptName.
+  Definition rclear_asm (l : list RegName) : list asm_code :=
+  (fun r => mov r 0) <$> l.
+  Definition rclear (l : list RegName) : list instr :=
+    Eval cbn in assemble (rclear_asm l).
+  Definition rclear_instrs (l : list RegName) : list Word :=
+    encodeInstrsW (rclear l).
+  Definition rclear_instrs' (l : list RegName) : list Word
+    := (fun r => (encodeInstrW (machine_base.Mov r (inl 0%Z)))) <$> l.
 
-  Definition dom_arg_rmap (nargs : nat) : gset RegName :=
-    match nargs with
-    | 0 => ∅
-    | 1 => {[ ca0 ]}
-    | 2 => {[ ca0 ; ca1 ]}
-    | 3 => {[ ca0 ; ca1 ; ca2 ]}
-    | 4 => {[ ca0 ; ca1 ; ca2 ; ca3 ]}
-    | 5 => {[ ca0 ; ca1 ; ca2 ; ca3 ; ca4 ]}
-    | 6 => {[ ca0 ; ca1 ; ca2 ; ca3 ; ca4 ; ca5 ]}
-    | _ => {[ ca0 ; ca1 ; ca2 ; ca3 ; ca4 ; ca5 ; ct0 ]}
-    end.
-
-
-  Definition is_arg_rmap (rmap : Reg) (nargs : nat) :=
-    dom rmap = dom_arg_rmap nargs.
-
+  Definition registers_pre_call_skip : list RegName :=
+    [ca0;ca1;ca2;ca3;ca4;ca5;ct0].
+  Definition clear_registers_pre_call_skip_asm : list asm_code :=
+    [ jmp ct2 ] ++ rclear_asm registers_pre_call_skip.
+  Definition clear_registers_pre_call_skip : list instr :=
+    Eval compute in assemble clear_registers_pre_call_skip_asm.
   Definition clear_registers_pre_call_skip_instrs : list Word :=
-    encodeInstrsW [ Jmp ct2;
-                    Mov ca0 0%Z;
-                    Mov ca1 0%Z;
-                    Mov ca2 0%Z;
-                    Mov ca3 0%Z;
-                    Mov ca4 0%Z;
-                    Mov ca5 0%Z;
-                    Mov ct0 0%Z].
+    encodeInstrsW clear_registers_pre_call_skip.
 
+  Definition registers_pre_call : list RegName :=
+    [cnull;
+     ctp; ct1; ct2; cs0; cs1; ca6; ca7;
+     cs2; cs3; cs4; cs5; cs6; cs7; cs8; cs9; cs10; cs11;
+     ct3; ct4; ct5; ct6
+    ].
+  Definition clear_registers_pre_call_asm : list asm_code :=
+    rclear_asm registers_pre_call.
+  Definition clear_registers_pre_call : list instr :=
+    Eval compute in assemble clear_registers_pre_call_asm.
   Definition clear_registers_pre_call_instrs : list Word :=
-    encodeInstrsW [
-        Mov cnull 0%Z;
-        Mov ctp 0%Z;
-        Mov ct1 0%Z;
-        Mov ct2 0%Z;
-        Mov cs0 0%Z;
-        Mov cs1 0%Z;
-        Mov ca6 0%Z;
-        Mov ca7 0%Z;
-        Mov cs2 0%Z;
-        Mov cs3 0%Z;
-        Mov cs4 0%Z;
-        Mov cs5 0%Z;
-        Mov cs6 0%Z;
-        Mov cs7 0%Z;
-        Mov cs8 0%Z;
-        Mov cs9 0%Z;
-        Mov cs10 0%Z;
-        Mov cs11 0%Z;
-        Mov ct3 0%Z;
-        Mov ct4 0%Z;
-        Mov ct5 0%Z;
-        Mov ct6 0%Z
-      ].
+    encodeInstrsW clear_registers_pre_call.
 
+  Definition registers_post_call : list RegName :=
+    [ct0; cnull;
+     ctp; ct1; ct2; ct3; ct4; ct5; ct6;
+     ca2; ca3; ca4; ca5; ca6; ca7;
+     cs2; cs3; cs4; cs5; cs6; cs7; cs8; cs9; cs10; cs11
+    ].
+  Definition clear_registers_post_call_asm : list asm_code :=
+    rclear_asm registers_post_call.
+  Definition clear_registers_post_call : list instr :=
+    Eval compute in assemble clear_registers_post_call_asm.
   Definition clear_registers_post_call_instrs : list Word :=
-    encodeInstrsW [
-        Mov ct0 0%Z;
-        Mov cnull 0%Z;
-        Mov ctp 0%Z;
-        Mov ct1 0%Z;
-        Mov ct2 0%Z;
-        Mov ct3 0%Z;
-        Mov ct4 0%Z;
-        Mov ct5 0%Z;
-        Mov ct6 0%Z;
-        Mov ca2 0%Z;
-        Mov ca3 0%Z;
-        Mov ca4 0%Z;
-        Mov ca5 0%Z;
-        Mov ca6 0%Z;
-        Mov ca7 0%Z;
-        Mov cs2 0%Z;
-        Mov cs3 0%Z;
-        Mov cs4 0%Z;
-        Mov cs5 0%Z;
-        Mov cs6 0%Z;
-        Mov cs7 0%Z;
-        Mov cs8 0%Z;
-        Mov cs9 0%Z;
-        Mov cs10 0%Z;
-        Mov cs11 0%Z
-      ].
-
-  Lemma clear_registers_post_call_spec
-    (pc_p : Perm) (pc_g : Locality) (pc_b pc_e pc_a : Addr)
-    (rmap : Reg) φ :
-    executeAllowed pc_p = true ->
-    SubBounds pc_b pc_e pc_a (pc_a ^+ length clear_registers_post_call_instrs)%a ->
-
-    dom rmap = all_registers_s ∖ {[ PC ; cra ; cgp ; csp ; cs0 ; cs1 ; ca0 ; ca1 ]} ->
-
-    ( PC ↦ᵣ WCap pc_p pc_g pc_b pc_e pc_a
-      ∗ ( [∗ map] r↦w ∈ rmap, r ↦ᵣ w )
-      ∗ codefrag pc_a clear_registers_post_call_instrs
-      ∗ ▷ ( (∃ (rmap' : Reg),
-              ⌜ dom rmap' = all_registers_s ∖ {[ PC ; cra ; cgp ; csp ; cs0 ; cs1 ; ca0 ; ca1 ]} ⌝
-              ∗ PC ↦ᵣ WCap pc_p pc_g pc_b pc_e (pc_a ^+ length clear_registers_post_call_instrs)%a
-              ∗ ( [∗ map] r↦w ∈ rmap', r ↦ᵣ w ∗ ⌜ w = WInt 0 ⌝ )
-              ∗ codefrag pc_a clear_registers_post_call_instrs)
-               -∗ WP Seq (Instr Executable) {{ φ }})
-    )
-    ⊢ WP Seq (Instr Executable) {{ φ }}%I.
-  Proof.
-    iIntros (Hx Hbounds Hdom) "(HPC & Hregs & Hcode & Hcont)".
-
-    iAssert ([∗ map] r↦_ ∈ rmap, ∃ w, r ↦ᵣ w)%I with "[Hregs]" as "Hregs".
-    { iApply (big_sepM_mono with "Hregs"). intros. eauto. }
-
-    iDestruct (big_sepM_dom with "Hregs") as "Hregs".
-    rewrite Hdom.
-
-    iDestruct (big_sepS_delete _ _ ct0 with "Hregs") as "[[% ?] Hregs]";[set_solver|].
-    iDestruct (big_sepS_delete _ _ cnull with "Hregs") as "[[% ?] Hregs]";[set_solver|].
-    iDestruct (big_sepS_delete _ _ ctp with "Hregs") as "[[% ?] Hregs]";[set_solver|].
-    iDestruct (big_sepS_delete _ _ ct1 with "Hregs") as "[[% ?] Hregs]";[set_solver|].
-    iDestruct (big_sepS_delete _ _ ct2 with "Hregs") as "[[% ?] Hregs]";[set_solver|].
-    iDestruct (big_sepS_delete _ _ ct3 with "Hregs") as "[[% ?] Hregs]";[set_solver|].
-    iDestruct (big_sepS_delete _ _ ct4 with "Hregs") as "[[% ?] Hregs]";[set_solver|].
-    iDestruct (big_sepS_delete _ _ ct5 with "Hregs") as "[[% ?] Hregs]";[set_solver|].
-    iDestruct (big_sepS_delete _ _ ct6 with "Hregs") as "[[% ?] Hregs]";[set_solver|].
-    iDestruct (big_sepS_delete _ _ ca2 with "Hregs") as "[[% ?] Hregs]";[set_solver|].
-    iDestruct (big_sepS_delete _ _ ca3 with "Hregs") as "[[% ?] Hregs]";[set_solver|].
-    iDestruct (big_sepS_delete _ _ ca4 with "Hregs") as "[[% ?] Hregs]";[set_solver|].
-    iDestruct (big_sepS_delete _ _ ca5 with "Hregs") as "[[% ?] Hregs]";[set_solver|].
-    iDestruct (big_sepS_delete _ _ ca6 with "Hregs") as "[[% ?] Hregs]";[set_solver|].
-    iDestruct (big_sepS_delete _ _ ca7 with "Hregs") as "[[% ?] Hregs]";[set_solver|].
-    iDestruct (big_sepS_delete _ _ cs2 with "Hregs") as "[[% ?] Hregs]";[set_solver|].
-    iDestruct (big_sepS_delete _ _ cs3 with "Hregs") as "[[% ?] Hregs]";[set_solver|].
-    iDestruct (big_sepS_delete _ _ cs4 with "Hregs") as "[[% ?] Hregs]";[set_solver|].
-    iDestruct (big_sepS_delete _ _ cs5 with "Hregs") as "[[% ?] Hregs]";[set_solver|].
-    iDestruct (big_sepS_delete _ _ cs6 with "Hregs") as "[[% ?] Hregs]";[set_solver|].
-    iDestruct (big_sepS_delete _ _ cs7 with "Hregs") as "[[% ?] Hregs]";[set_solver|].
-    iDestruct (big_sepS_delete _ _ cs8 with "Hregs") as "[[% ?] Hregs]";[set_solver|].
-    iDestruct (big_sepS_delete _ _ cs9 with "Hregs") as "[[% ?] Hregs]";[set_solver|].
-    iDestruct (big_sepS_delete _ _ cs10 with "Hregs") as "[[% ?] Hregs]";[set_solver|].
-    iDestruct (big_sepS_delete _ _ cs11 with "Hregs") as "[[% ?] _]";[set_solver|].
-
-    codefrag_facts "Hcode". clear H0.
-    iGo "Hcode".
-
-    iApply "Hcont".
-    iExists
-      (<[ct0:=_]> (<[cnull:=_]> (<[ctp:=_]> (<[ct1:=_]>(<[ct2:=_]>(<[ct3:=_]>(<[ct4:=_]>(<[ct5:=_]>(<[ct6:=_]>(<[ca2:=_]>(<[ca3:=_]>(<[ca4:=_]>(<[ca5:=_]>(<[ca6:=_]>(<[ca7:=_]> (<[cs2:=_]> (<[cs3:=_]> (<[cs4:=_]> (<[cs5:=_]> (<[cs6:=_]> (<[cs7:=_]> (<[cs8:=_]> (<[cs9:=_]> (<[cs10:=_]> (<[cs11:=_]> ∅))))))))))))))))))))))))).
-    repeat (rewrite big_sepM_insert;[|by simplify_map_eq]).
-    iFrame. iSplit.
-    { iPureIntro. rewrite !dom_insert_L. set_solver. }
-    repeat (iSplit;[done|]). done.
-  Qed.
-
-
-End ClearRegistersMacro.
+    encodeInstrsW clear_registers_post_call.
+End ClearStackMacro.
