theories/case_studies/lse_downward/lse_spec.v
@@ -1,7 +1,7 @@
 From iris.proofmode Require Import proofmode.
 From cap_machine Require Import region_invariants_revocation interp_weakening monotone.
 From cap_machine Require Import rules logrel logrel_extra monotone proofmode register_tactics.
-From cap_machine Require Import fetch assert switcher switcher_spec_call.
+From cap_machine Require Import fetch_spec assert_spec switcher switcher_spec_call.
 From cap_machine Require Import lse lse_spec_closure.
 From cap_machine Require Import proofmode.
 
