theories/case_studies/macros/assert.v
@@ -1,150 +1,46 @@
-From iris.proofmode Require Import proofmode.
-From cap_machine Require Import logrel rules proofmode.
+From cap_machine Require Import machine_parameters assembler.
 From cap_machine Require Import fetch.
 
-(* Assert routine *)
+Section Assert_Code.
+  Import Asm_Griotte.
+  Local Coercion Z.of_nat : nat >-> Z.
+  Context `{MP: MachineParameters}.
 
-(* Maintains a flag storing whether an assert has failed. *)
-
-Section Assert_subroutine.
-  Context
-    {Σ : gFunctors}
-      {ceriseg: ceriseG Σ}
-      {nainv: logrel_na_invs Σ}
-      {MP: MachineParameters}
-  .
+  (* Maintains a flag storing whether an assert has failed. *)
 
   (* Asserts (ct0 == ct1). Jumps back to cra.
      Clobbers cra, ct0, ct1.
    *)
-  Definition assert_subroutine_instrs :=
-    encodeInstrsW [
-      Sub ct0 ct0 ct1;
-      Jnz 4 ct0;
-      (* success case *)
-      Mov ct0 0;
-      Mov ct1 0;
-      JmpCap cra; (* return *)
-      (* failure case *)
-      Mov ct1 PC; (* pointer to cap: *)
-      Lea ct1 7; (* pointer to cap: *)
-      Load ct1 ct1;
-      Store ct1 1;
-      Mov ct0 0;
-      Mov ct1 0;
-      JmpCap cra (* return *)
+  Definition assert_subroutine_asm_pre :=
+    [
+      sub ct0 ct0 ct1;
+      jnz ("assert_fail")%asm ct0;
+      #"assert_success";
+      mov ct0 0;
+      mov ct1 0;
+      jmpcap cra; (* return *)
+      #"assert_fail";
+      mov ct1 PC;
+      lea ct1 ("cap_flag"+1)%asm; (* pointer to cap: *)
+      load ct1 ct1;
+      store ct1 1;
+      mov ct0 0;
+      mov ct1 0;
+      jmpcap cra;
+      #"cap_flag"
+       (* cap: (RW, flag, end, flag) *)
+       (* flag: <0 or 1> *)
+       (* end*)
     ].
-  (* followed in memory by:
-    cap: (RW, flag, end, flag)
-    flag: <0 or 1>
-    end:
-  *)
 
-  Definition assert_inv (b_assert e_assert a_flag : Addr) : iProp Σ :=
-    (∃ cap_addr,
-       codefrag b_assert assert_subroutine_instrs ∗
-       ⌜(b_assert + length assert_subroutine_instrs)%a = Some cap_addr⌝ ∗
-       ⌜(cap_addr + 1)%a = Some e_assert⌝ ∗
-       ⌜is_Some (a_flag + 1)%a⌝ ∗
-       cap_addr ↦ₐ WCap RW Global a_flag (a_flag ^+1)%a a_flag).
-
-  Lemma assert_subroutine_spec
-    (pc_g : Locality) (pc_b pc_e a_flag : Addr)
-    ( n1 n2 flag : Z ) ( wret : Word)
-    (N : namespace) (E : coPset) (φ : language.val cap_lang -> iProp Σ) :
-    ↑N ⊆ E →
-    (  na_inv logrel_nais N (assert_inv pc_b pc_e a_flag)
-     ∗ na_own logrel_nais E
-     ∗ PC ↦ᵣ WCap RX pc_g pc_b pc_e pc_b
-     ∗ cra ↦ᵣ wret
-     ∗ ct0 ↦ᵣ WInt n1
-     ∗ ct1 ↦ᵣ WInt n2
-     ∗ a_flag ↦ₐ WInt flag
-     ∗ ▷ (na_own logrel_nais E
-          ∗ PC ↦ᵣ updatePcPerm wret
-          ∗ cra ↦ᵣ wret
-          ∗ ct0 ↦ᵣ WInt 0
-          ∗ ct1 ↦ᵣ WInt 0
-          ∗ a_flag ↦ₐ WInt (if (n1 =? n2)%Z then flag else 1%Z)
-          -∗ WP Seq (Instr Executable) {{ φ }})
-     ⊢ WP Seq (Instr Executable) {{ φ }})%I.
-  Proof.
-    iIntros (HNE) "(#Hinv & Hna & HPC & Hrdst & Hct0 & Hct1 & Hflag & Hφ)".
-    iMod (na_inv_acc with "Hinv Hna") as "(>Hassert & Hna & Hinv_close)"; auto.
-    iDestruct "Hassert" as (cap_addr) "(Hprog & %Hcap & %Hpc_e & %He_flag & Hcap)".
-    destruct He_flag as [e_flag He_flag].
-    rewrite /assert_subroutine_instrs.
-    codefrag_facts "Hprog". rename H into HcontProg.
-    assert (SubBounds pc_b pc_e
-              pc_b (pc_b ^+ length assert_subroutine_instrs)%a)
-      as HsubBounds by solve_addr.
-    iInstr "Hprog".
-    destruct (decide (n1 = n2)) as [Heq|Heq].
-    { (* n1 = n2 *)
-      subst n2. rewrite (_: n1 - n1 = 0)%Z; last lia.
-      iGo "Hprog".
-      iMod ("Hinv_close" with "[Hprog Hcap $Hna]") as "Hna".
-      { iExists _. iNext. iFrame. iPureIntro. repeat split; solve_addr. }
-
-      iApply "Hφ". iFrame. rewrite Z.eqb_refl //. }
-    { (* n1 ≠ n2 *)
-      iInstr "Hprog". { assert (n1 - n2 ≠ 0)%Z by lia. congruence. }
-      iInstr "Hprog".
-      iInstr "Hprog".
-      rewrite (_: (pc_b ^+ 12)%a = cap_addr); [|solve_addr].
-      iInstr "Hprog"; first solve_addr.
-      iInstr "Hprog"; first solve_addr.
-      iGo "Hprog".
-      iMod ("Hinv_close" with "[Hprog Hcap $Hna]") as "Hna".
-      { iExists _. iNext. iFrame. iPureIntro. repeat split; solve_addr. }
-      iApply "Hφ". iFrame. rewrite (_: (n1 =? n2)%Z = false) //.
-      by apply Z.eqb_neq. }
-  Qed.
-
-  Lemma assert_subroutine_success_spec
-    (pc_g : Locality) (pc_b pc_e a_flag : Addr)
-    ( n1 n2 flag : Z ) ( wret : Word)
-    (N : namespace) (E : coPset) (φ : language.val cap_lang -> iProp Σ) :
-    ↑N ⊆ E →
-    n1 = n2 →
-    (  na_inv logrel_nais N (assert_inv pc_b pc_e a_flag)
-     ∗ na_own logrel_nais E
-     ∗ PC ↦ᵣ WCap RX pc_g pc_b pc_e pc_b
-     ∗ cra ↦ᵣ wret
-     ∗ ct0 ↦ᵣ WInt n1
-     ∗ ct1 ↦ᵣ WInt n2
-     ∗ ▷ (na_own logrel_nais E
-          ∗ PC ↦ᵣ updatePcPerm wret
-          ∗ cra ↦ᵣ wret
-          ∗ ct0 ↦ᵣ WInt 0%Z
-          ∗ ct1 ↦ᵣ WInt 0%Z
-          -∗ WP Seq (Instr Executable) {{ φ }})
-     ⊢ WP Seq (Instr Executable) {{ φ }})%I.
-  Proof.
-    iIntros (HNE Heq) "(#Hinv & Hna & HPC & Hrdst & Hct0 & Hct1 & Hφ)".
-    iMod (na_inv_acc with "Hinv Hna") as "(>Hassert & Hna & Hinv_close)"; auto.
-    iDestruct "Hassert" as (cap_addr) "(Hprog & %Hcap & %Hflag & %He & Hcap)".
-    rewrite /assert_subroutine_instrs. codefrag_facts "Hprog".
-    assert (SubBounds pc_b pc_e
-              pc_b (pc_b ^+ length assert_subroutine_instrs)%a)
-      as HsubBounds by solve_addr.
-    iInstr "Hprog".
-    rewrite (_: n1 - n2 = 0)%Z; last lia.
-    iGo "Hprog".
-    iMod ("Hinv_close" with "[Hprog Hcap $Hna]") as "Hna".
-    { iExists _. iNext. iFrame. iPureIntro. repeat split; solve_addr. }
-    iApply "Hφ". iFrame.
-  Qed.
-
-End Assert_subroutine.
-
-Section Assert.
-  Context
-    {Σ : gFunctors}
-      {ceriseg: ceriseG Σ}
-      {nainv: logrel_na_invs Σ}
-      {MP: MachineParameters}
-  .
+  Definition assert_subroutine_asm_env :=
+    Eval vm_compute in (compute_asm_code_env (assert_subroutine_asm_pre)).2.
+  Definition assert_subroutine_asm :=
+    Eval compute in resolve_labels_macros assert_subroutine_asm_pre assert_subroutine_asm_env.
+  Definition assert_subroutine : list instr :=
+    Eval compute in assemble assert_subroutine_asm.
+  Definition assert_subroutine_instrs : list Word :=
+    encodeInstrsW assert_subroutine.
 
   (* assert macros:
    - fetch the assert entry point an the n-th position in the import table
@@ -152,75 +48,20 @@ Section Assert.
 
    - rdst, rscratch1 and rscratch2 are all clobbered
    *)
-  Definition assert_instrs (n : Z) (rdst rscratch1 rscratch2 : RegName) :=
-    fetch_instrs n rdst rscratch1 rscratch2 ++
-    encodeInstrsW [
-      Mov rscratch1 cra;
-      Jalr cra rdst;
-      Mov cra rscratch1;
-      Mov rscratch1 0%Z;
-      Mov rdst 0%Z
+  Definition assert_asm (n : Z) (rdst rscratch1 rscratch2 : RegName) :=
+    [ fetch_asm n rdst rscratch1 rscratch2
+      ;
+      [
+        mov rscratch1 cra;
+        jalr cra rdst;
+        mov cra rscratch1;
+        mov rscratch1 0;
+        mov rdst 0
+      ]
     ].
 
-  Lemma assert_success_spec
-    (n : Z) (rdst rscratch1 rscratch2 : RegName)
-    (pc_g : Locality) (pc_p : Perm) (pc_b pc_e pc_a : Addr)
-    (g_assert : Locality) (b_assert e_assert a_flag : Addr)
-    (n1 n2 : Z) (wdst wcra w1 w2 : Word)
-    (N : namespace) (E : coPset) (φ : language.val cap_lang -> iProp Σ) :
-
-    let assert_macro := assert_instrs n rdst rscratch1 rscratch2 in
-    let a_last := (pc_a ^+ length assert_macro)%a in
-    executeAllowed pc_p = true →
-    SubBounds pc_b pc_e pc_a a_last →
-    withinBounds pc_b pc_e (pc_b ^+ n)%a = true ->
-
-    ↑N ⊆ E →
-    n1 = n2 →
-    (  na_inv logrel_nais N (assert_inv b_assert e_assert a_flag)
-     ∗ na_own logrel_nais E
-     ∗ PC ↦ᵣ WCap pc_p pc_g pc_b pc_e pc_a
-     ∗ rdst ↦ᵣ wdst
-     ∗ rscratch1 ↦ᵣ w1
-     ∗ rscratch2 ↦ᵣ w2
-     ∗ cra ↦ᵣ wcra
-     ∗ ct0 ↦ᵣ WInt n1
-     ∗ ct1 ↦ᵣ WInt n2
-     ∗ codefrag pc_a assert_macro
-     ∗ (pc_b ^+ n)%a ↦ₐ (WSentry RX g_assert b_assert e_assert b_assert)
-     ∗ ▷ (na_own logrel_nais E
-          ∗ PC ↦ᵣ WCap pc_p pc_g pc_b pc_e a_last
-          ∗ rdst ↦ᵣ WInt 0
-          ∗ rscratch1 ↦ᵣ WInt 0
-          ∗ rscratch2 ↦ᵣ WInt 0
-          ∗ cra ↦ᵣ wcra
-          ∗ ct0 ↦ᵣ WInt 0
-          ∗ ct1 ↦ᵣ WInt 0
-          ∗ codefrag pc_a assert_macro
-          ∗ (pc_b ^+ n)%a ↦ₐ (WSentry RX g_assert b_assert e_assert b_assert)
-          -∗ WP Seq (Instr Executable) {{ φ }})
-     ⊢ WP Seq (Instr Executable) {{ φ }})%I.
-  Proof.
-    intros assert_macro a_last; subst assert_macro a_last.
-    iIntros (Hpc_exec HsubBounds Hinbounds HNE Heq)
-      "(#Hinv & Hna & HPC & Hrdst & Hrscratch1 & Hrscratch2 & Hcra & Hct0 & Hct1 & Hcode & Hpc_bn & Hφ)".
-    codefrag_facts "Hcode".
-    rewrite /assert_instrs.
-    focus_block_0 "Hcode" as "Hfetch" "Hcont".
-    iApply (fetch_spec with "[-]"); eauto; iFrame.
-    iNext; iIntros "(HPC & Hrdst & Hrscratch1 & Hrscratch2 & Hfetch & Hpc_bn)".
-    unfocus_block "Hfetch" "Hcont" as "Hcode".
-    focus_block 1 "Hcode" as a_assert Ha_assert "Hassert" "Hcont".
-    iGo "Hassert".
-    rewrite load_word_sentry.
-    iEval (cbn) in "HPC".
-    iApply (assert_subroutine_success_spec with "[-]"); eauto; iFrame "#∗".
-    iNext; iIntros "(Hna & HPC & Hcra & Hct0 & Hct1)".
-    iEval (cbn) in "HPC".
-    iGo "Hassert".
-    unfocus_block "Hassert" "Hcont" as "Hcode".
-    replace (a_assert ^+ 5)%a with (pc_a ^+ 14)%a by solve_addr.
-    iApply "Hφ"; iFrame.
-  Qed.
-
-End Assert.
+  Definition assembled_assert (n : Z) (rdst rscratch1 rscratch2 : RegName) :=
+    Eval compute in assemble_block (assert_asm n rdst rscratch1 rscratch2).
+  Definition assert_instrs (n : Z) (rdst rscratch1 rscratch2 : RegName) : list Word :=
+    concat (encodeInstrsW <$> (assembled_assert n rdst rscratch1 rscratch2)).
+End Assert_Code.
