theories/case_studies/macros/fetch_spec.v
@@ -1,0 +1,50 @@
+From iris.proofmode Require Import proofmode.
+From cap_machine Require Import rules proofmode.
+From cap_machine Require Export fetch.
+
+Section Fetch.
+  Context
+    {Σ : gFunctors}
+      {ceriseg: ceriseG Σ}
+      {MP: MachineParameters}
+  .
+  Lemma fetch_spec
+    (n : Z) (rdst rscratch1 rscratch2 : RegName)
+    (pc_p : Perm) (pc_g : Locality) (pc_b pc_e pc_a : Addr)
+    (wentry wdst w1 w2 : Word)
+    (φ : language.val cap_lang → iPropI Σ) :
+
+    let fetch_ := (fetch_instrs n rdst rscratch1 rscratch2) in
+    let a_last := (pc_a ^+ length fetch_)%a in
+    executeAllowed pc_p = true →
+    SubBounds pc_b pc_e pc_a a_last →
+    withinBounds pc_b pc_e (pc_b ^+ n)%a = true ->
+
+    ▷ PC ↦ᵣ WCap pc_p pc_g pc_b pc_e pc_a
+    ∗ ▷ rdst ↦ᵣ wdst
+    ∗ ▷ rscratch1 ↦ᵣ w1
+    ∗ ▷ rscratch2 ↦ᵣ w2
+    ∗ ▷ codefrag pc_a fetch_
+    ∗ ▷ (pc_b ^+ n)%a ↦ₐ wentry
+    ∗ ▷ (PC ↦ᵣ WCap pc_p pc_g pc_b pc_e a_last
+         ∗ rdst ↦ᵣ load_word pc_p wentry
+         ∗ rscratch1 ↦ᵣ WInt 0%Z
+         ∗ rscratch2 ↦ᵣ WInt 0%Z
+         ∗ codefrag pc_a fetch_
+         ∗ (pc_b ^+ n)%a ↦ₐ wentry
+         -∗ WP Seq (Instr Executable) {{ φ }})
+    ⊢ WP Seq (Instr Executable) {{ φ }}.
+  Proof.
+    intros fetch a_last ; subst fetch a_last.
+    iIntros (Hvpc Hcont Hpc_n)
+      "(>HPC & >Hrdst & >Hrscratch1 & >Hrscratch2 & >Hprog & >Hpc_bn & Hφ)".
+    iDestruct (big_sepL2_length with "Hprog") as %Hlength.
+    codefrag_facts "Hprog".
+    rename H into HcontRegion; clear H0.
+    assert ((pc_a + (pc_b - pc_a))%a = Some pc_b) as Hlea;[solve_addr|].
+    assert ((pc_b + n)%a = Some (pc_b ^+ n)%a) as Hpc_bn;[solve_addr|].
+    iGo "Hprog".
+    iApply "Hφ"; iFrame.
+  Qed.
+
+End Fetch.
