theories/switcher/clear_registers_spec.v
@@ -1,0 +1,177 @@
+From iris.algebra Require Import frac.
+From iris.proofmode Require Import proofmode.
+From cap_machine Require Import memory_region rules proofmode.
+From iris.program_logic Require Export weakestpre.
+From cap_machine Require Export cap_lang seal_store region_invariants.
+From iris.algebra Require Export gmap agree auth excl_auth.
+From iris.base_logic Require Export invariants na_invariants saved_prop.
+From cap_machine Require Import rules_base.
+From cap_machine Require Export clear_registers.
+
+
+Section ClearRegistersMacro.
+  Context
+    {Σ:gFunctors}
+    {ceriseg:ceriseG Σ}
+    {sealsg: sealStoreG Σ}
+    {Cname : CmptNameG}
+    {stsg : STSG Addr region_type Σ}
+    {heapg : heapGS Σ}
+    `{MP: MachineParameters}.
+
+  Implicit Types W : WORLD.
+  Implicit Types C : CmptName.
+
+  Definition dom_arg_rmap (nargs : nat) : gset RegName :=
+    let rargs := [ca0 ; ca1 ; ca2 ; ca3 ; ca4 ; ca5 ; ct0] in
+    list_to_set (firstn nargs rargs).
+
+  Definition is_arg_rmap (rmap : Reg) (nargs : nat) :=
+    dom rmap = dom_arg_rmap nargs.
+
+  Lemma rclear_spec
+    (pc_p : Perm) (pc_g : Locality) (pc_b pc_e pc_a : Addr)
+    (l : list RegName)
+    (rmap : Reg) φ :
+    l ≠ [] ->
+    executeAllowed pc_p = true ->
+    SubBounds pc_b pc_e pc_a (pc_a ^+ length (rclear_instrs' l ))%a ->
+
+    dom rmap = list_to_set l  ->
+
+    ( PC ↦ᵣ WCap pc_p pc_g pc_b pc_e pc_a
+      ∗ ( [∗ map] r↦w ∈ rmap, r ↦ᵣ w )
+      ∗ codefrag pc_a (rclear_instrs' l)
+      ∗ ▷ ( (∃ (rmap' : Reg),
+              ⌜ dom rmap' = list_to_set l ⌝
+              ∗ PC ↦ᵣ WCap pc_p pc_g pc_b pc_e (pc_a ^+ length (rclear_instrs' l ))%a
+              ∗ ( [∗ map] r↦w ∈ rmap', r ↦ᵣ w ∗ ⌜ w = WInt 0 ⌝ )
+              ∗ codefrag pc_a (rclear_instrs' l))
+               -∗ WP Seq (Instr Executable) {{ φ }})
+    )
+    ⊢ WP Seq (Instr Executable) {{ φ }}%I.
+  Proof.
+    iIntros (Hne Hx Hbounds Hdom) "(HPC & Hregs & Hcode & Hcont)".
+    iRevert (Hbounds Hdom).
+    iInduction (l) as [|r l] "IH" forall (rmap pc_a); iIntros (Hbounds Hrdom); first congruence.
+
+    cbn [list_to_set] in Hrdom.
+    assert (is_Some (rmap !! r)) as [rv Hr].
+    { apply elem_of_dom; rewrite Hrdom; set_solver. }
+    iDestruct (big_sepM_delete _ _ r with "Hregs") as "[Hr Hregs]"; eauto.
+    cbn.
+    codefrag_facts "Hcode".
+
+    iInstr "Hcode".
+    { transitivity (Some (pc_a ^+ 1)%a); auto; solve_addr. }
+    destruct (decide (l = [])).
+    { subst l. iApply "Hcont". iFrame.
+      replace (delete r rmap) with (∅ : Reg).
+      2: { symmetry.
+           rewrite -dom_empty_iff_L.
+           rewrite dom_delete_L.
+           rewrite Hrdom.
+           set_solver.
+         }
+      iExists (<[r := WInt 0]> ∅).
+      iSplit; cycle 1.
+      + iDestruct (big_sepM_insert (fun r w => r ↦ᵣ w ∗ ⌜ w = WInt 0⌝ )%I ∅ r with "[Hr Hregs]") as "H".
+        { done. }
+        { iFrame. iSplit; done. }
+        iFrame "H".
+      + iPureIntro ; set_solver.
+    }
+
+   iAssert (codefrag (pc_a ^+ 1)%a (rclear_instrs' l) ∗
+             (codefrag (pc_a ^+ 1)%a (rclear_instrs' l) -∗ codefrag pc_a (rclear_instrs' (r :: l))))%I
+    with "[Hcode]" as "[Hcode Hcls]".
+    { cbn. unfold codefrag. rewrite (region_pointsto_cons _ (pc_a ^+ 1)%a). 2,3: solve_addr.
+      iDestruct "Hcode" as "[? Hr]".
+      rewrite (_: ((pc_a ^+ 1) ^+ (length (rclear_instrs' l)))%a =
+                    (pc_a ^+ (S (length (rclear_instrs' l))))%a). 2: solve_addr.
+      iFrame. eauto. }
+
+    match goal with H : SubBounds _ _ _ _ |- _ =>
+      rewrite (_: (pc_a ^+ (length (rclear_instrs' (r :: l))))%a =
+                  ((pc_a ^+ 1)%a ^+ length (rclear_instrs' l))%a) in H |- *
+    end.
+    2: { unfold rclear_instrs'; cbn; solve_addr. }
+
+    destruct (decide (r ∈ l)).
+    - iDestruct (big_sepM_insert _ _ r with "[Hr $Hregs]") as "Hregs".
+      { by rewrite lookup_delete//. }
+      { by iFrame. }
+      iApply ("IH" with "[] HPC Hregs Hcode [Hcont Hcls]"); eauto.
+      { iNext.
+        iIntros "H"; iDestruct "H" as (rmap' Hdom_rmap')  "(HPC & Hregs & Hcode)".
+        iApply "Hcont"; iFrame.
+        iDestruct ("Hcls" with "Hcode") as "$".
+        iPureIntro; set_solver.
+      }
+      { iPureIntro; solve_pure_addr. }
+      {  iPureIntro. rewrite insert_delete_insert. set_solver. }
+    - iApply ("IH" with "[] HPC Hregs Hcode [Hcont Hcls Hr]"); eauto.
+      { iNext.
+        iIntros "H"; iDestruct "H" as (rmap' Hdom_rmap')  "(HPC & Hregs & Hcode)".
+        iDestruct (big_sepM_insert _ _ r with "[Hr $Hregs]") as "Hregs".
+        { rewrite -not_elem_of_dom Hdom_rmap'; set_solver. }
+        { iFrame. done. }
+        iApply "Hcont"; iFrame.
+        iDestruct ("Hcls" with "Hcode") as "$".
+        iPureIntro; set_solver.
+      }
+      { iPureIntro; solve_pure_addr. }
+      {  iPureIntro; set_solver. }
+  Qed.
+
+  Lemma clear_registers_post_call_spec
+    (pc_p : Perm) (pc_g : Locality) (pc_b pc_e pc_a : Addr)
+    (rmap : Reg) φ :
+    executeAllowed pc_p = true ->
+    SubBounds pc_b pc_e pc_a (pc_a ^+ length clear_registers_post_call_instrs)%a ->
+
+    dom rmap = all_registers_s ∖ {[ PC ; cra ; cgp ; csp ; cs0 ; cs1 ; ca0 ; ca1 ]} ->
+
+    ( PC ↦ᵣ WCap pc_p pc_g pc_b pc_e pc_a
+      ∗ ( [∗ map] r↦w ∈ rmap, r ↦ᵣ w )
+      ∗ codefrag pc_a clear_registers_post_call_instrs
+      ∗ ▷ ( (∃ (rmap' : Reg),
+              ⌜ dom rmap' = all_registers_s ∖ {[ PC ; cra ; cgp ; csp ; cs0 ; cs1 ; ca0 ; ca1 ]} ⌝
+              ∗ PC ↦ᵣ WCap pc_p pc_g pc_b pc_e (pc_a ^+ length clear_registers_post_call_instrs)%a
+              ∗ ( [∗ map] r↦w ∈ rmap', r ↦ᵣ w ∗ ⌜ w = WInt 0 ⌝ )
+              ∗ codefrag pc_a clear_registers_post_call_instrs)
+               -∗ WP Seq (Instr Executable) {{ φ }})
+    )
+    ⊢ WP Seq (Instr Executable) {{ φ }}%I.
+  Proof.
+    iIntros (Hx Hbounds Hdom) "(HPC & Hregs & Hcode & Hcont)".
+    iApply (rclear_spec _ _ _ _ _ registers_post_call); eauto.
+    iFrame.
+  Qed.
+
+  Lemma clear_registers_pre_call_spec
+    (pc_p : Perm) (pc_g : Locality) (pc_b pc_e pc_a : Addr)
+    (rmap : Reg) φ :
+    executeAllowed pc_p = true ->
+    SubBounds pc_b pc_e pc_a (pc_a ^+ length clear_registers_pre_call_instrs)%a ->
+
+    dom rmap = all_registers_s ∖ (dom_arg_rmap 8 ∪ {[ PC ; cra ; cgp ; csp ]}) ->
+
+    ( PC ↦ᵣ WCap pc_p pc_g pc_b pc_e pc_a
+      ∗ ( [∗ map] r↦w ∈ rmap, r ↦ᵣ w )
+      ∗ codefrag pc_a clear_registers_pre_call_instrs
+      ∗ ▷ ( (∃ (rmap' : Reg),
+              ⌜ dom rmap' = all_registers_s ∖ (dom_arg_rmap 8 ∪ {[ PC ; cra ; cgp ; csp ]}) ⌝
+              ∗ PC ↦ᵣ WCap pc_p pc_g pc_b pc_e (pc_a ^+ length clear_registers_pre_call_instrs)%a
+              ∗ ( [∗ map] r↦w ∈ rmap', r ↦ᵣ w ∗ ⌜ w = WInt 0 ⌝ )
+              ∗ codefrag pc_a clear_registers_pre_call_instrs)
+               -∗ WP Seq (Instr Executable) {{ φ }})
+    )
+    ⊢ WP Seq (Instr Executable) {{ φ }}%I.
+  Proof.
+    iIntros (Hx Hbounds Hdom) "(HPC & Hregs & Hcode & Hcont)".
+    iApply (rclear_spec _ _ _ _ _ registers_pre_call); eauto.
+    iFrame.
+  Qed.
+
+End ClearRegistersMacro.
